Add solution for Pset6

pset6/Pset6.v
@@ -58,7 +58,10 @@ Inductive cmd :=
 
 (** Notations *)
 
+Declare Scope cmd_scope.
 Delimit Scope cmd_scope with cmd.
+
+Declare Scope arith_scope.
 
 Coercion Const : nat >-> arith.
 Coercion Var : var >-> arith.
@@ -143,29 +146,159 @@ Fixpoint interp (e : arith) (v : valuation) : nat :=
      sanity check!
  *)
 
-Definition result : Type.
-Admitted.
+Inductive result : Type :=
+  | Terminated (v: valuation)
+  | Aborted.
 
-Definition eval : valuation -> cmd -> result -> Prop.
-Admitted.
+Inductive eval : valuation -> cmd -> result -> Prop :=
+  | EvalAssign : forall v x a,
+      eval v (Assign x a) (Terminated (v $+ (x, interp a v)))
+  | EvalSkip : forall v,
+      eval v Skip (Terminated v)
+  | EvalSeqAborted : forall v0 cmd0 cmd1,
+      eval v0 cmd0 Aborted -> eval v0 (Seq cmd0 cmd1) Aborted
+  | EvalSeqSuccess : forall v0 cmd0 v1 cmd1 res,
+      eval v0 cmd0 (Terminated v1) -> eval v1 cmd1 res -> eval v0 (Seq cmd0 cmd1) res
+  | EvalChoose0 : forall v cmd0 cmd1 res,
+      eval v cmd0 res -> eval v (Choose cmd0 cmd1) res
+  | EvalChoose1 : forall v cmd0 cmd1 res,
+      eval v cmd1 res -> eval v (Choose cmd0 cmd1) res
+  | EvalIfFalse : forall v a cmd1 cmd0 res,
+      interp a v = O -> eval v cmd0 res -> eval v (If a cmd1 cmd0) res
+  | EvalIfTrue : forall v a cmd1 cmd0 res,
+      interp a v <> O -> eval v cmd1 res -> eval v (If a cmd1 cmd0) res
+  | EvalWhileFalse : forall v a cmd,
+      interp a v = O -> eval v (While a cmd) (Terminated v)
+  | EvalWhileTrueAborted : forall v a cmd,
+      interp a v <> O -> eval v cmd Aborted -> eval v (While a cmd) Aborted
+  | EvalWhileTrueSuccess : forall v0 a cmd v1 res,
+      interp a v0 <> O -> eval v0 cmd (Terminated v1) -> eval v1 (While a cmd) res -> eval v0 (While a cmd) res
+  | EvalAbort : forall v,
+      eval v Abort Aborted.
 
-Definition big_aborted : result -> Prop.
-Admitted.
+Definition big_aborted : result -> Prop := fun r => r = Aborted.
 
 (* As an optional sanity check, you may attempt to
  * prove that your big-step semantics behaves appropriately
- * for an example program:
+ * for an example program: *)
  
+Lemma extract_y : forall (a b c: nat), ($0 $+ ("target", a) $+ ("x", b) $+ ("y", c)) $? "y" = Some c.
+Proof.
+  intros a b c.
+  exact (lookup_add_eq ($0 $+ ("target", a) $+ ("x", b)) c (eq_refl "y")).
+Qed.
+
+Lemma extract_x : forall (a b c: nat), ($0 $+ ("target", a) $+ ("x", b) $+ ("y", c)) $? "x" = Some b.
+Proof.
+  assert ("x" <> "y") as x_not_y.
+    intros abs.
+    discriminate abs.
+  intros a b c.
+  rewrite (lookup_add_ne ($0 $+ ("target", a) $+ ("x", b)) c x_not_y).
+  exact (lookup_add_eq ($0 $+ ("target", a)) b (eq_refl "x")).
+Qed.
+
+Lemma extract_target : forall (a b c: nat), ($0 $+ ("target", a) $+ ("x", b) $+ ("y", c)) $? "target" = Some a.
+Proof.
+  assert ("target" <> "y") as target_not_y.
+    intros abs.
+    discriminate abs.
+  assert ("target" <> "x") as target_not_x.
+    intros abs.
+    discriminate abs.
+  intros a b c.
+  rewrite (lookup_add_ne ($0 $+ ("target", a) $+ ("x", b)) c target_not_y).
+  rewrite (lookup_add_ne ($0 $+ ("target", a)) b target_not_x).
+  exact (lookup_add_eq ($0) a (eq_refl "target")).
+Qed.
+
 Example test_prog1_reachable :
   exists res, eval $0 (test_prog1 5) res /\ big_aborted res.
 Proof.
-Admitted.
+  refine (ex_intro _ Aborted (conj _ (eq_refl Aborted))).
+  refine (EvalSeqSuccess $0 _ _ _ Aborted _ _).
+  refine (EvalSeqSuccess _ _ _ _ _ _ _).
+  refine (EvalSeqSuccess _ _ _ _ _ _ _).
+  refine (EvalAssign _ _ _).
+  refine (EvalChoose0 _ _ _ _ (EvalAssign _ _ _)).
+  refine (EvalChoose1 _ _ _ _ (EvalAssign _ _ _)).
+  refine (EvalIfTrue _ _ _ _ _ _ _).
+  simpl.
+  rewrite (extract_x 8 3 5).
+  rewrite (extract_y 8 3 5).
+  rewrite (extract_target 8 3 5).
+  discriminate.
+  exact (EvalAbort _).
+Qed.
 
 Example test_prog1_unreachable :
   forall res, eval $0 (test_prog1 6) res -> big_aborted res -> False.
 Proof.
-Admitted.
-*)
+  intros res evaluation res_value.
+  invert res_value.
+  invert evaluation.
+  (* Show that we cannot abort before the If *)
+    invert H1.
+    invert H2.
+    invert H1.
+    invert H5.
+    invert H4.
+    invert H4.
+    invert H5.
+    invert H4.
+    invert H4.
+  (* Show that the If will not abort *)
+    invert H2.
+    invert H3.
+    invert H6.
+    invert H7.
+    (* left left *)
+      invert H5.
+      invert H6.
+      invert H2.
+      invert H4.
+      invert H6.
+      simpl in H5.
+      rewrite (extract_x 8 3 1) in H5.
+      rewrite (extract_y 8 3 1) in H5.
+      rewrite (extract_target 8 3 1) in H5.
+      exact (H5 (eq_refl O)).
+    (* right left *)
+      invert H5.
+      invert H6.
+      invert H2.
+      invert H4.
+      invert H6.
+      simpl in H5.
+      rewrite (extract_x 8 4 1) in H5.
+      rewrite (extract_y 8 4 1) in H5.
+      rewrite (extract_target 8 4 1) in H5.
+      exact (H5 (eq_refl O)).
+    invert H7.
+    (* left right *)
+      invert H5.
+      invert H6.
+      invert H2.
+      invert H4.
+      invert H6.
+      simpl in H5.
+      rewrite (extract_x 8 3 6) in H5.
+      rewrite (extract_y 8 3 6) in H5.
+      rewrite (extract_target 8 3 6) in H5.
+      exact (H5 (eq_refl O)).
+    (* right right *)
+      invert H5.
+      invert H6.
+      invert H2.
+      invert H4.
+      invert H6.
+      simpl in H5.
+      rewrite (extract_x 8 4 6) in H5.
+      rewrite (extract_y 8 4 6) in H5.
+      rewrite (extract_target 8 4 6) in H5.
+      exact (H5 (eq_refl O)).
+Qed.
+
 
 
   (** ** Part 2: Small-step deterministic operational semantics *)
@@ -214,36 +347,435 @@ Admitted.
    a good sanity check!
  *)
 
-Definition state : Type.
-Admitted.
+(* From the instructions:
+   forall s1 s2 s2', step s1 s2 -> step s1 s2' -> s2 = s2'
+   If we want states to contain some current valuation(s),
+   we need another axiom about valuations.
+   That axiom could be derived from fmap_ext if we incorporate the fact that
+   valuations would always operate over the same finite set of strings.
+   We'll just add a new axiom here though, to be able to actually write s2 = s2' *)
+Axiom valuation_dec : forall x y : valuation, sumbool (x = y) (x <> y).
 
-Definition step : state -> state -> Prop.
-Admitted.
+(*
 
-Definition init : valuation -> cmd -> state.
-Admitted.
+   > (It is actually possible to define a semantics that always "finds" aborts,
+   > even if some branches of nondeterminism diverge!  However, the proof of that
+   > variant would likely be significantly more complicated, and we haven't tried
+   > it ourselves.)
+   Let's do it!
+*)
 
-Definition small_aborted : state -> Prop.
-Admitted.
+Inductive singular_state :=
+  | SRunning (v: valuation) (l: list cmd)
+  | SDone (r: result).
 
-Definition small_terminated : state -> Prop.
-Admitted.
+Definition state := list singular_state.
 
+Definition singular_step (s: singular_state) : list singular_state := match s with
+  | SRunning v nil => [SDone (Terminated v)]
+  | SRunning v ((Assign x a)::q) => [SRunning (v $+ (x, interp a v)) q]
+  | SRunning v (Skip::q) => [SRunning v q]
+  | SRunning v ((Seq c1 c2)::q) => [SRunning v (c1::c2::q)]
+  | SRunning v ((Choose c1 c2)::q) => [SRunning v (c1::q); SRunning v (c2::q)]
+  | SRunning v ((If a c1 c0)::q) => match interp a v with
+    | O => [SRunning v (c0::q)]
+    | _ => [SRunning v (c1::q)]
+    end
+  | SRunning v ((While a c)::q) => match interp a v with
+    | O => [SRunning v q]
+    | _ => [SRunning v (c::(While a c)::q)]
+    end
+  | SRunning v (Abort::q) => [SDone Aborted]
+  | SDone (Terminated v) => [SDone (Terminated v)]
+  | SDone Aborted => [SDone Aborted]
+  end.
+
+Definition full_step (s: state) : state := flat_map singular_step s.
+
+Definition step : state -> state -> Prop :=
+  fun x y => y = full_step x.
+
+Definition init : valuation -> cmd -> state :=
+    fun (v: valuation) (c: cmd) => [SRunning v [c]].
+
+Lemma arith_dec : forall x y : arith, sumbool (x = y) (x <> y).
+Proof.
+  decide equality.
+  exact (Nat.eq_dec n n0).
+  exact (string_dec s s0).
+Qed.
+
+Lemma cmd_dec : forall x y : cmd, sumbool (x = y) (x <> y).
+Proof.
+  decide equality.
+  exact (arith_dec a a0).
+  exact (string_dec s s0).
+  exact (arith_dec a a0).
+  exact (arith_dec a a0).
+Qed.
+
+Lemma result_dec : forall x y : result, sumbool (x = y) (x <> y).
+Proof.
+  intros x y; destruct x, y; decide equality; exact (valuation_dec _ _).
+Qed.
+
+Lemma state_dec : forall x y : singular_state, sumbool (x = y) (x <> y).
+Proof.
+  decide equality.
+  exact (list_eq_dec cmd_dec _ _).
+  exact (valuation_dec _ _).
+  exact (result_dec _ _).
+Qed.
+
+(*
+Inductive small_aborted : state -> Prop :=
+  | FirstAborted : forall q, small_aborted (SAborted::q)
+  | TailAborted : forall x q, small_aborted q -> small_aborted (x::q).
+Theorem small_aborted_in : forall s : state, small_aborted s <-> In SAborted s.
+Proof. (* should probably have defined it with In in the first place... *)
+  
+Qed.
+*)
+Definition small_aborted (s:state) : Prop := In (SDone Aborted) s.
+Fixpoint small_aborted_bool (s:state) : bool := match s with
+  | nil => false
+  | (SRunning _ _)::q => small_aborted_bool q
+  | (SDone (Terminated _))::q => small_aborted_bool q
+  | (SDone Aborted)::_ => true
+  end.
+Theorem small_aborted_equiv : forall st : state, small_aborted st <-> small_aborted_bool st = true.
+Proof.
+  intro st.
+  elim st.
+  (* [] *)
+    split.
+      intro absurd; elim absurd.
+      discriminate.
+  (* a::q *)
+    intros a q rec.
+    split.
+    (* small_aborted (a :: q) -> small_aborted_bool (a :: q) = true *)
+      intro H; elim H.
+        intro a_aborted; rewrite a_aborted; trivial.
+        elim a.
+          intros v l; unfold small_aborted_bool; exact (proj1 rec).
+          intro r; elim r.
+            exact (fun _ => (proj1 rec)).
+            reflexivity.
+    (* small_aborted_bool (a :: q) = true -> small_aborted (a :: q) *)
+      elim a.
+        intros v l H; exact (or_intror (proj2 rec H)).
+        intro r; elim r.
+          exact (fun _ H => or_intror (proj2 rec H)).
+          exact (fun _ => or_introl (eq_refl (SDone Aborted))).
+Qed.
+
+Fixpoint small_terminated_bool (s:state) : bool := match s with
+  | nil => true
+  | (SRunning _ _)::q => false
+  | (SDone (Terminated _))::q => small_terminated_bool q
+  | (SDone Aborted)::_ => false
+  end.
+Definition small_terminated (s:state) : Prop := small_terminated_bool s = true.
+Theorem small_terminated_only_terminated : forall (s:state) (res:singular_state),
+    small_terminated s -> In res s -> exists v:valuation, res = SDone (Terminated v).
+Proof.
+  intro s; elim s; clear s.
+  (* [] *)
+    intros res taut absurd; elim absurd.
+  intro a; elim a; clear a.
+  (* (SRunning v l)::q *)
+    intros v l q rec res absurd; discriminate absurd.
+  intro r; elim r; clear r.
+  (* (SDone (Terminated v))::q *)
+    intros v q rec res H1 H2; elim H2; clear H2.
+      intro result; exists v; exact (eq_sym result).
+      exact (rec _ H1).
+  (* (SDone Aborted)::q *)
+    intros l rec res absurd; discriminate absurd.
+Qed.
+
+Fixpoint iterate (A:Type) (F:A -> A) (n:nat){struct n} : A -> A := match n with
+  | O => fun x => x
+  | S m => fun x => iterate A F m (F x)
+  end.
+Definition do_steps (n:nat) : state -> state := iterate state full_step n.
+Theorem do_steps_ex : forall n : nat, forall st : state, step^* st (do_steps n st).
+Proof.
+  intros n.
+  elim n.
+  (* Base case *)
+    intros st.
+    exact (TrcRefl step st).
+  (* Recursion *)
+    intros m H st.
+    refine (TrcFront st (eq_refl (full_step st)) _).
+    exact (H (full_step st)).
+Qed.
+Theorem do_steps_find : forall st1 st2 : state, step^* st1 st2 -> exists n:nat, st2 = do_steps n st1.
+Proof.
+  intros st1 st2 H.
+  elim H.
+  (* Base case *)
+    intro x.
+    exact (ex_intro _ O (eq_refl x)).
+  (* Recursion *)
+    intros x y z xy yz rec.
+    invert rec.
+    invert xy.
+    exact (ex_intro _ (S x0) (eq_refl _)).
+Qed.
+Lemma do_steps_split0 : forall (n:nat) (st:state), full_step (do_steps n st) = do_steps n (full_step st).
+Proof.
+  intro n; elim n; clear n; [reflexivity|].
+  intros n rec st.
+  replace (do_steps (S n) st) with (do_steps n (full_step st)) by reflexivity.
+  rewrite (rec _).
+  reflexivity.
+Qed.
+Theorem do_steps_split : forall (n m:nat) (st:state), do_steps n (do_steps m st) = do_steps (n+m) st.
+Proof.
+  intro n; elim n; clear n; [reflexivity|].
+  intros n rec m st.
+  replace (do_steps (S n) (do_steps m st))
+      with (do_steps n (full_step (do_steps m st))) by reflexivity.
+  rewrite (do_steps_split0 _ _).
+  rewrite (rec _ _).
+  reflexivity.
+Qed.
+
+(* Two lemmas borrowed from newer versions of Coq;
+   might have to comment out and remove implicit arguments further down. *)
+Lemma flat_map_concat_map : forall A B, forall f:A->list B, forall l,
+    flat_map f l = concat (map f l).
+Proof.
+  induction l as [|x l IH]; simpl.
+  - reflexivity.
+  - rewrite IH; reflexivity.
+Qed.
+Lemma flat_map_app : forall A B, forall f:A->list B, forall l1 l2,
+    flat_map f (l1 ++ l2) = flat_map f l1 ++ flat_map f l2.
+Proof.
+  intros A B f l1 l2.
+  now rewrite !flat_map_concat_map, map_app, concat_app.
+Qed.
+(* End of the borrowing :-) *)
+
+Theorem step_split :
+    forall (n:nat) (l1 l2: list singular_state),
+    do_steps n (l1 ++ l2) = (do_steps n l1) ++ (do_steps n l2).
+Proof.
+  intro n; elim n.
+  (* Base case *)
+    reflexivity.
+  (* Recursion *)
+    clear n; intros n rec l1 l2.
+    replace (do_steps (S n) (l1 ++ l2)) with (do_steps n (flat_map singular_step (l1 ++ l2))) by reflexivity.
+    replace (do_steps (S n) l1) with (do_steps n (flat_map singular_step l1)) by reflexivity.
+    replace (do_steps (S n) l2) with (do_steps n (flat_map singular_step l2)) by reflexivity.
+    rewrite (flat_map_app _ _ singular_step l1 l2).
+    exact (rec _ _).
+Qed.
+
+Theorem empty_future : forall st : state, step ^* nil st -> st = nil.
+Proof.
+  intros st H.
+  induct H.
+  (* Base case *)
+    reflexivity.
+  (* Recursion *)
+    compute in H.
+    rewrite H in IHtrc.
+    exact (IHtrc (JMeq.JMeq_refl nil)).
+Qed.
+Lemma terminated_split : forall l1 l2 : list singular_state,
+    small_terminated l1 /\ small_terminated l2 <-> small_terminated (l1 ++ l2).
+Proof.
+  intro l1; elim l1.
+  (* Base case *)
+    split.
+      intros [useless H]; exact H.
+      exact (fun H => conj (eq_refl true) H).
+  (* Recursion *)
+    intros a q rec l2; elim a.
+    (* SRunning *)
+      intros v c; split; [intros [absurd Hl2]|intro absurd]; discriminate absurd.
+    intro r; elim r.
+    (* SDone (Terminated v) *)
+      intros v; exact (rec l2).
+    (* SDone Abort *)
+      split; [intros [absurd Hl2]|intro absurd]; discriminate absurd.
+Qed.
+Theorem terminated_future : forall st1 st2 : state,
+    small_terminated st1 -> step ^* st1 st2 -> small_terminated st2.
+Proof.
+  assert (
+      forall n:nat, forall st1:state,
+      small_terminated st1 -> small_terminated (do_steps n st1)
+  ) as recgoal.
+    intro n; elim n.
+    (* Base case *)
+      exact (fun _ H => H).
+    (* Recursion *)
+      clear n; intros n rec st1; elim st1.
+      (* [] *)
+        rewrite (empty_future _ (do_steps_ex (S n) nil)); reflexivity.
+      (* a::q *)
+        intro a; elim a.
+        (* SRunning *)
+          intros v c q rec2 absurd; discriminate absurd.
+        intro r; elim r.
+        (* SDone (Terminated v) *)
+          intros v q rec2 Hq.
+          replace (SDone (Terminated v) :: q) with ([SDone (Terminated v)] ++ q) by reflexivity.
+          rewrite (step_split _ _ _).
+          refine (proj1 (terminated_split _ _) (conj (rec _ _) (rec2 Hq))); reflexivity.
+        (* SDone Aborted *)
+          intros q rec2 absurd; discriminate absurd.
+  (* Back to the main goal *)
+  intros st1 st2 base evol.
+  elim (do_steps_find st1 st2 evol).
+  intros n Hst2; rewrite Hst2; exact (recgoal n st1 base).
+Qed.
+
+Lemma terminated_not_aborted : forall s:state, small_terminated s -> ~ (small_aborted s).
+Proof.
+  intro s; elim s.
+  (* [] *)
+    intros useless absurd; elim absurd.
+  (* a::q *)
+    intro a; elim a.
+    (* SRunning v c *)
+      intros v c q rec absurd; discriminate absurd.
+    intro r; elim r.
+    (* SDone (Terminated v) *)
+      intros v c rec H absurd.
+      elim (in_inv absurd); [discriminate | exact (rec H)].
+    (* SDone Aborted *)
+      discriminate.
+Qed.
 
 (* As an optional sanity check, you may attempt to
  * prove that your small-step semantics behaves appropriately
- * for an example program:
+ * for an example program: *)
+
+Lemma test_lookup_y : forall t x y : nat, ($0 $+ ("target", t) $+ ("x", x) $+ ("y", y)) $? "y" = Some y.
+Proof.
+  intros t x y.
+  exact (lookup_add_eq _ _ (eq_refl "y")).
+Qed.
+Lemma test_lookup_x : forall t x y : nat, ($0 $+ ("target", t) $+ ("x", x) $+ ("y", y)) $? "x" = Some x.
+Proof.
+  intros t x y.
+  assert ("x" <> "y") as H.
+    discriminate.
+  rewrite (lookup_add_ne _ _ H).
+  exact (lookup_add_eq _ _ (eq_refl "x")).
+Qed.
+Lemma test_lookup_target : forall t x y : nat, ($0 $+ ("target", t) $+ ("x", x) $+ ("y", y)) $? "target" = Some t.
+Proof.
+  intros t x y.
+  assert ("target" <> "y") as Hy.
+    discriminate.
+  rewrite (lookup_add_ne _ _ Hy).
+  assert ("target" <> "x") as Hx.
+    discriminate.
+  rewrite (lookup_add_ne _ _ Hx).
+  exact (lookup_add_eq _ _ (eq_refl "target")).
+Qed.
 
 Example test_prog1_reachable_small :
   exists st, step^* (init $0 (test_prog1 5)) st /\ small_aborted st.
 Proof.
-Admitted.
+  refine (ex_intro _ (do_steps 10 (init $0 (test_prog1 5))) _).
+  split.
+  (* left side *)
+    exact (do_steps_ex 10 (init $0 (test_prog1 5))).
+  (* right side *)
+    compute.
+    rewrite
+      (test_lookup_x 8 3 1), (test_lookup_x 8 3 5), (test_lookup_x 8 4 1), (test_lookup_x 8 4 5),
+      (test_lookup_y 8 3 1), (test_lookup_y 8 3 5), (test_lookup_y 8 4 1), (test_lookup_y 8 4 5),
+      (test_lookup_target 8 3 1), (test_lookup_target 8 3 5),
+      (test_lookup_target 8 4 1), (test_lookup_target 8 4 5).
+    compute.
+    exact (or_intror (or_introl (eq_refl (SDone Aborted)))).
+Qed.
 
 Example test_prog1_unreachable_small :
   forall st, step^* (init $0 (test_prog1 6)) st -> small_aborted st -> False.
 Proof.
-Admitted.
-*)
+  intros st H absurd.
+  pose (my_absurd := proj1 (small_aborted_equiv st) absurd).
+  invert H.
+  (* step 0 *)
+    discriminate my_absurd.
+  invert H0.
+  invert H1.
+  (* step 1 *)
+    discriminate my_absurd.
+  invert H.
+  invert H0.
+  (* step 2 *)
+    discriminate my_absurd.
+  invert H.
+  invert H1.
+  (* step 3 *)
+    discriminate my_absurd.
+  invert H.
+  invert H0.
+  (* step 4 *)
+    discriminate my_absurd.
+  invert H.
+  invert H1.
+  (* step 5 *)
+    discriminate my_absurd.
+  invert H.
+  invert H0.
+  (* step 6 *)
+    discriminate my_absurd.
+  invert H.
+  invert H1.
+  (* step 7 *)
+    discriminate my_absurd.
+  invert H.
+  invert H0.
+  (* step 8 *)
+    discriminate my_absurd.
+  invert H.
+  replace
+      (full_step (full_step (full_step (full_step
+      (full_step (full_step (full_step (full_step
+      (full_step (init $0 (test_prog1 6)))))))))))
+    with
+      [SRunning ($0 $+ ("target", 8) $+ ("x", 3) $+ ("y", 1)) [Skip];
+       SRunning ($0 $+ ("target", 8) $+ ("x", 3) $+ ("y", 6)) [Skip];
+       SRunning ($0 $+ ("target", 8) $+ ("x", 4) $+ ("y", 1)) [Skip];
+       SRunning ($0 $+ ("target", 8) $+ ("x", 4) $+ ("y", 6)) [Skip]]
+    in H1.
+  (* Proving the final steps *)
+    invert H1.
+    (* Step 9 *)
+      discriminate my_absurd.
+    invert H.
+    invert H0.
+    (* Step 10 *)
+      discriminate my_absurd.
+    invert H.
+    (* Remaining steps - nil state *)
+    refine (
+        (terminated_not_aborted _ (terminated_future _ _ _ H1))
+        (proj2 (small_aborted_equiv _) my_absurd)); reflexivity.
+  (* Proving the rewrite *)
+    compute.
+    rewrite
+        (test_lookup_x 8 3 1), (test_lookup_x 8 3 6), (test_lookup_x 8 4 1), (test_lookup_x 8 4 6),
+        (test_lookup_y 8 3 1), (test_lookup_y 8 3 6), (test_lookup_y 8 4 1), (test_lookup_y 8 4 6),
+        (test_lookup_target 8 3 1), (test_lookup_target 8 3 6),
+        (test_lookup_target 8 4 1), (test_lookup_target 8 4 6).
+    reflexivity.
+Qed.
+
 
 (** ** Part 3: Connection between big- and small-step semantics *)
 
@@ -254,14 +786,885 @@ Admitted.
  * potentially abort.
  *)
 
+Lemma eval_dec : forall m:nat, m=O \/ exists p:nat, m=S p.
+Proof.
+  intro m; destruct m;
+      [ exact (or_introl (eq_refl O)) | exact (or_intror (ex_intro _ m (eq_refl (S m)))) ].
+Qed.
+Lemma abort_interrupts : forall n:nat, forall (c1 c2:list cmd) (v:valuation),
+  small_aborted (do_steps n [SRunning v c1]) -> small_aborted (do_steps n [SRunning v (c1 ++ c2)]).
+Proof.
+  intro n; elim n.
+  (* Base case *)
+    intros c1 c2 v absurd; discriminate (proj1 (small_aborted_equiv _) absurd).
+  (* Recursion *)
+    clear n; intros n rec c1; elim c1.
+    (* [] *)
+      intros c2 v absurd.
+      replace (do_steps (S n) [SRunning v []]) with (do_steps n [SDone (Terminated v)]) in absurd by reflexivity.
+      assert (small_terminated [SDone (Terminated v)]) as taut.
+        reflexivity.
+      elim (terminated_not_aborted _ (terminated_future _ _ taut (do_steps_ex n [SDone (Terminated v)])) absurd).
+    intro a; elim a.
+    (* (Assign va a)::q *)
+      exact (fun _ _ _ _ _ _ H => rec _ _ _ H).
+    (* Skip::q *)
+      exact (fun _ _ _ _ H => rec _ _ _ H).
+    (* (Seq ca cb)::q *)
+      exact (fun _ _ _ _ _ _ _ _ H => rec _ _ _ H).
+    (* (Choose ca cb)::q *)
+      intros ca rec2 cb rec3 q rec4 c2 v H.
+      replace (do_steps (S n) [SRunning v (((ca <|> cb)%cmd :: q) ++ c2)])
+          with (do_steps n ((SRunning v (ca::q ++ c2))::[SRunning v (cb::q ++ c2)])) by reflexivity.
+      replace (do_steps (S n) [SRunning v ((ca <|> cb)%cmd :: q)])
+          with (do_steps n ((SRunning v (ca::q))::[SRunning v (cb::q)])) in H by reflexivity.
+      replace ((SRunning v (ca::q ++ c2))::[SRunning v (cb::q ++ c2)])
+          with ([SRunning v (ca::q ++ c2)] ++ [SRunning v (cb::q ++ c2)]) by reflexivity.
+      replace ((SRunning v (ca::q))::[SRunning v (cb::q)])
+          with ([SRunning v (ca::q)] ++ [SRunning v (cb::q)]) in H by reflexivity.
+      rewrite (step_split n [SRunning v (ca::q ++ c2)] [SRunning v (cb::q ++ c2)]).
+      rewrite (step_split n [SRunning v (ca::q)] [SRunning v (cb::q)]) in H.
+      refine (in_or_app _ _ _ _).
+      elim (in_app_or _ _ _ H); intro Hcab;
+          [ exact (or_introl (rec _ _ _ Hcab)) | exact (or_intror (rec _ _ _ Hcab)) ].
+    (* If e ca cb *)
+      intros e ca rec2 cb rec3 q rec4 c2 v.
+      replace (do_steps (S n) [SRunning v (((if_ e then ca else cb)%cmd :: q) ++ c2)])
+        with (do_steps n (full_step [SRunning v (((if_ e then ca else cb)%cmd :: q) ++ c2)])) by reflexivity.
+      replace (do_steps (S n) [SRunning v (((if_ e then ca else cb)%cmd :: q))])
+        with (do_steps n (full_step [SRunning v (((if_ e then ca else cb)%cmd :: q))])) by reflexivity.
+      replace (((if_ e then ca else cb)%cmd :: q) ++ c2)
+        with ([(if_ e then ca else cb)%cmd] ++ (q ++ c2)) by exact ((app_assoc _ _ _)).
+      replace ([(if_ e then ca else cb)%cmd] ++ (q ++ c2))
+        with (((if_ e then ca else cb)%cmd)::(q ++ c2)) by reflexivity.
+      unfold full_step, singular_step, flat_map.
+      replace (match interp e v with
+          | 0 => [SRunning v (cb :: q ++ c2)]
+          | S _ => [SRunning v (ca :: q ++ c2)]
+          end ++ [])
+        with (match interp e v with
+          | 0 => [SRunning v (cb :: q ++ c2)]
+          | S _ => [SRunning v (ca :: q ++ c2)]
+          end) by exact (eq_sym (app_nil_r _)).
+      replace (match interp e v with
+          | 0 => [SRunning v (cb :: q)]
+          | S _ => [SRunning v (ca :: q)]
+          end ++ [])
+        with (match interp e v with
+          | 0 => [SRunning v (cb :: q)]
+          | S _ => [SRunning v (ca :: q)]
+          end) by exact (eq_sym (app_nil_r _)).
+      elim (eval_dec (interp e v)).
+      (* Then branch *)
+        intros ev; rewrite ev; exact (rec _ _ _).
+      (* Else branch *)
+        intros evex; elim evex; intros p ev; rewrite ev; exact (rec _ _ _).
+    (* While e c *)
+      intros e c rec2 q rec3 c2 v.
+      replace (do_steps (S n) [SRunning v (((while e do c)%cmd :: q) ++ c2)])
+        with (do_steps n (full_step [SRunning v (((while e do c)%cmd :: q) ++ c2)])) by reflexivity.
+      replace (do_steps (S n) [SRunning v (((while e do c)%cmd :: q))])
+        with (do_steps n (full_step [SRunning v (((while e do c)%cmd :: q))])) by reflexivity.
+      replace (((while e do c)%cmd :: q) ++ c2)
+        with ([(while e do c)%cmd] ++ (q ++ c2)) by exact ((app_assoc _ _ _)).
+      replace ([(while e do c)%cmd] ++ (q ++ c2))
+        with (((while e do c)%cmd)::(q ++ c2)) by reflexivity.
+      unfold full_step, singular_step, flat_map.
+      replace (match interp e v with
+          | 0 => [SRunning v (q ++ c2)]
+          | S _ => [SRunning v (c::(while e do c)%cmd::q ++ c2)]
+          end ++ [])
+        with (match interp e v with
+          | 0 => [SRunning v (q ++ c2)]
+          | S _ => [SRunning v (c::(while e do c)%cmd::q ++ c2)]
+          end) by exact (eq_sym (app_nil_r _)).
+      replace (match interp e v with
+          | 0 => [SRunning v q]
+          | S _ => [SRunning v (c::(while e do c)%cmd::q)]
+          end ++ [])
+        with (match interp e v with
+          | 0 => [SRunning v q]
+          | S _ => [SRunning v (c::(while e do c)%cmd::q)]
+          end) by exact (eq_sym (app_nil_r _)).
+      elim (eval_dec (interp e v)).
+      (* Do branch *)
+        intros ev; rewrite ev; exact (rec _ _ _).
+      (* Done branch *)
+        intros evex; elim evex; intros p ev; rewrite ev; exact (rec _ _ _).
+    (* Abort *)
+      assert (forall m:nat, do_steps m [SDone Aborted] = [SDone Aborted]) as aborted_stays.
+        intro m; elim m; [ reflexivity | exact (fun _ H => H) ].
+      intros q rec2 c2 v H.
+      replace (do_steps (S n) [SRunning v ((Abort :: q) ++ c2)])
+          with (do_steps n ([SDone Aborted])) by reflexivity.
+      rewrite (aborted_stays n).
+      exact (or_introl (eq_refl _)).
+Qed.
+
+Lemma keep_pace : forall (a:cmd) (q:list cmd) (v1 v2:valuation),
+    ~ In (SDone (Terminated v2)) (full_step [SRunning v1 (a::q)]).
+Proof.
+  intro a; elim a; clear a.
+  (* Assign *)
+    intros s a q v1 v2 absurd; invert absurd; [ discriminate H | elim H ].
+  (* Skip *)
+    intros q v1 v2 absurd; invert absurd; [ discriminate H | elim H ].
+  (* Seq *)
+    intros c1 rec1 c2 rec2 q v1 v2 absurd; invert absurd; [ discriminate H | elim H ].
+  (* Choose *)
+    intros c1 rec1 c2 rec2 q v1 v2 absurd; invert absurd; [ discriminate H | elim H ].
+      discriminate.
+      intro H2; elim H2.
+  (* If *)
+    intros a c1 rec1 c2 rec2 q v1 v2.
+    replace (full_step [SRunning v1 ((if_ a then c1 else c2)%cmd :: q)])
+        with (match interp a v1 with
+        | O => [SRunning v1 (c2::q)]
+        | S _ => [SRunning v1 (c1::q)]
+        end) by exact (eq_sym (app_nil_r _)).
+    elim (eval_dec (interp a v1)); [|intro Hp; elim Hp; clear Hp; intro p];
+        intros H absurd; rewrite H in absurd; elim absurd; clear absurd; intro absurd;
+        [ discriminate absurd | elim absurd | discriminate absurd | elim absurd ].
+  (* While *)
+    intros a c rec q v1 v2.
+    replace (full_step [SRunning v1 ((while a do c)%cmd :: q)])
+        with (match interp a v1 with
+        | O => [SRunning v1 q]
+        | S _ => [SRunning v1 (c::(While a c)::q)]
+        end) by exact (eq_sym (app_nil_r _)).
+    elim (eval_dec (interp a v1)); [|intro Hp; elim Hp; clear Hp; intro p];
+        intros H absurd; rewrite H in absurd; elim absurd; clear absurd; intro absurd;
+        [ discriminate absurd | elim absurd | discriminate absurd | elim absurd ].
+  (* Abort *)
+    intros q v1 v2 absurd; elim absurd; clear absurd; intro absurd; [ discriminate absurd | elim absurd ].
+Qed.
+
+Lemma before_termination0 : forall (st:state) (v:valuation),
+    ~ In (SDone (Terminated v)) st
+      -> In (SDone (Terminated v)) (full_step st)
+      -> In (SRunning v []) st.
+Proof.
+  intro st; elim st; clear st.
+  (* [] *)
+    intros v taut absurd; elim (absurd).
+  assert (forall (a:singular_state) (q:list singular_state) (v:valuation),
+      In (SDone (Terminated v)) (full_step (a::q))
+        -> In (SDone (Terminated v)) (full_step [a]) \/ In (SDone (Terminated v)) (full_step q))
+      as my_rewrite.
+    intros a q v.
+    replace (full_step (a :: q)) with ((full_step [a]) ++ (full_step q))
+        by exact (eq_sym (flat_map_app _ _ singular_step _ _)).
+    exact (in_app_or _ _ _).
+  intro a; elim a; clear a.
+  intros v0 l0; elim l0; clear l0.
+  (* (SRunning v0 nil)::q *)
+    intros q rec v not_here here; elim (my_rewrite _ _ _ here).
+    (* a contains the terminaison *)
+      intro done_in; elim done_in; clear done_in; intro done_eq; invert done_eq.
+      exact (or_introl (eq_refl _)).
+    (* q contains the terminaison *)
+      intro H; refine (_ (rec _ (fun P => not_here (in_cons _ _ _ P)) H)).
+      exact (in_cons _ _ _).
+  (* (SRunning v0 ac::qc)::q *)
+    intros ac qc rec q rec2 v not_here here. elim (my_rewrite _ _ _ here).
+    (* a contains the terminaison *)
+      intro absurd; elim (keep_pace _ _ _ _ absurd).
+    (* q contains the terminaison *)
+      intro H; refine (_ (rec2 _ (fun P => not_here (in_cons _ _ _ P)) H)).
+      exact (in_cons _ _ _).
+  intro r; elim r; clear r.
+  (* (SDone (Terminated v0))::q *)
+    intros v q rec v0 v0_not_v H; elim (valuation_dec v v0).
+      intro v_eq_v0; rewrite v_eq_v0 in v0_not_v; elim (v0_not_v (or_introl (eq_refl _))).
+      intro v_not_v0; right; elim (my_rewrite _ _ _ H).
+        intro absurd; elim absurd; clear absurd; intro absurd; invert absurd; elim (v_not_v0 (eq_refl _)).
+        exact (rec _ (fun P => v0_not_v (in_cons _ _ _ P))).
+  (* (SDone Abort)::q *)
+    intros q rec v not_here here; elim (my_rewrite _ _ _ here).
+      intro absurd; invert absurd; [ discriminate H | invert H ].
+      intro term_q; right; exact (rec _ (fun P => not_here (in_cons _ _ _ P)) term_q).
+Qed.
+Lemma before_termination : forall (n:nat) (st:state) (v:valuation),
+    ~ In (SDone (Terminated v)) st
+      -> In (SDone (Terminated v)) (do_steps n st)
+      -> exists m:nat, In (SRunning v nil) (do_steps m st).
+Proof.
+  (* Main goal: *)
+  intro n; elim n.
+  (* Base case *)
+    intros st v not_there there; elim (not_there there).
+  (* Recursion *)
+    clear n; intros n rec st v H0 H1.
+    elim (in_dec state_dec (SDone (Terminated v)) (full_step st)).
+    (* One step *)
+      intro H; exists O.
+      exact (before_termination0 _ _ H0 H).
+    (* More than one step *)
+      intro H; elim (rec _ _ H H1); intros m Hb; exists (S m); exact Hb.
+Qed.
+Lemma before_termination_or : forall (s:state) (v:valuation),
+    In (SDone (Terminated v)) (full_step s) -> In (SDone (Terminated v)) s \/ In (SRunning v nil) s.
+Proof.
+  intros s v; elim (in_dec state_dec (SDone (Terminated v)) s).
+    exact (fun P _ => or_introl P).
+    exact (fun H1 H2 => or_intror (before_termination0 _ _ H1 H2)).
+Qed.
+
+Lemma before_aborted (s:state) :
+    In (SDone Aborted) (full_step s)
+      -> In (SDone Aborted) s \/ exists v q, In (SRunning v (Abort::q)) s.
+Proof.
+  elim s; clear s.
+  (* [] *)
+    intro absurd; elim absurd.
+  intro a; elim a; clear a.
+  (* (SRunning v l)::q *)
+    intros v l q rec.
+    replace (full_step (SRunning v l :: q)) with (flat_map singular_step ([SRunning v l] ++ q)) by reflexivity.
+    rewrite (flat_map_app _ _ singular_step _ _).
+    intro H; elim (in_app_or _ _ _ H); clear H; intro H.
+    (* Abort from (SRunning v l) *)
+      destruct l; [ elim H; [ discriminate | intro absurd; elim absurd ] |].
+      destruct c.
+        elim H; [ discriminate | intro absurd; elim absurd ].  (* Assign *)
+        elim H; [ discriminate | intro absurd; elim absurd ].  (* Skip *)
+        elim H; [ discriminate | intro absurd; elim absurd ].  (* Seq *)
+        elim H; [ discriminate | intro absurd; elim absurd; clear absurd;
+            [ discriminate | intro absurd; elim absurd ] ].  (* Choose *)
+      (* If *)
+        replace (flat_map singular_step [SRunning v ((if_ a then c1 else c2)%cmd :: l)])
+            with (match interp a v with | O => [SRunning v (c2::l)] | _ => [SRunning v (c1::l)] end ++ [])
+            in H by reflexivity.
+        elim (eval_dec (interp a v)); intro interpeval;
+            [| elim interpeval; clear interpeval; intros p interpeval ];
+            rewrite interpeval in H;
+            elim H; [ discriminate | intro absurd; elim absurd | discriminate | intro absurd; elim absurd ].
+      (* While *)
+        replace (flat_map singular_step [SRunning v ((while a do c)%cmd :: l)])
+            with (match interp a v with | O => [SRunning v l] | _ => [SRunning v (c::(While a c)::l)] end ++ [])
+            in H by reflexivity.
+        elim (eval_dec (interp a v)); intro interpeval;
+            [| elim interpeval; clear interpeval; intros p interpeval ];
+            rewrite interpeval in H;
+            elim H; [ discriminate | intro absurd; elim absurd | discriminate | intro absurd; elim absurd ].
+      (* Abort *)
+        exact (or_intror (ex_intro _ v (ex_intro _ l (or_introl (eq_refl _))))).
+    (* Abort from q *)
+      elim (rec H); clear rec H; intro H.
+        exact (or_introl (in_cons _ _ _ H)).
+        elim H; clear H; intros v0 H; elim H; clear H; intros q0 H; right; exists v0, q0;
+            exact (in_cons _ _ _ H).
+  intro r; elim r; clear r.
+  (* (SDone (Terminated v))::q *)
+    intros v q rec.
+    replace (full_step (SDone (Terminated v) :: q))
+        with (flat_map singular_step ([SDone (Terminated v)] ++ q)) by reflexivity.
+    rewrite (flat_map_app _ _ singular_step _ _).
+    intro H; elim (in_app_or _ _ _ H); clear H; intro H;
+        [ elim H; clear H; [ discriminate | intro H; elim H ] |].
+    elim (rec H); clear rec H; intro H.
+      exact (or_introl (in_cons _ _ _ H)).
+      elim H; clear H; intros v0 H; elim H; clear H; intros q0 H; right; exists v0, q0;
+          exact (in_cons _ _ _ H).
+  (* (SDone Aborted)::q *)
+    exact (fun _ _ _ => or_introl (or_introl (eq_refl _))).
+Qed.
+
+Lemma before_running : forall (s:state) (v:valuation) (lc:list cmd),
+    In (SRunning v lc) (full_step s)
+      -> exists v0 lc0, In (SRunning v0 lc0) s /\ In (SRunning v lc) (full_step [SRunning v0 lc0]).
+Proof.
+  intro s; elim s; clear s; [ intros v lc absurd; elim absurd |].
+  intro a; elim a; clear a.
+  (* SRunning v l :: q *)
+    intros v l q rec v0 lc.
+    replace (full_step (SRunning v l :: q))
+        with (flat_map singular_step ([SRunning v l] ++ q)) by reflexivity.
+    rewrite (flat_map_app _ _ singular_step _ _).
+    intro H; elim (in_app_or _ _ _ H); clear H; intro H.
+      exists v, l; exact (conj (or_introl (eq_refl _)) H).
+      elim (rec _ _ H); clear rec H; intros v1 H; elim H; clear H; intros lc1 H.
+        exists v1, lc1; exact (conj (in_cons _ _ _ (proj1 H)) (proj2 H)).
+  (* SDone r :: q *)
+    intros r q rec v lc.
+    replace (full_step (SDone r :: q))
+        with (flat_map singular_step ([SDone r] ++ q)) by reflexivity.
+    rewrite (flat_map_app _ _ singular_step _ _).
+    intro H; elim (in_app_or _ _ _ H); clear H; intro H.
+      destruct r; elim H;
+          [ discriminate | intro absurd; elim absurd | discriminate | intro absurd; elim absurd ].
+      elim (rec _ _ H); clear rec H; intros v1 H; elim H; clear H; intros lc1 H.
+        exists v1, lc1; exact (conj (in_cons _ _ _ (proj1 H)) (proj2 H)).
+Qed.
+
+Lemma abort_const : forall m:nat, do_steps m [SDone Aborted] = [SDone Aborted].
+Proof.
+  intro m; elim m; clear m.
+    reflexivity.
+    intros m H; rewrite <- H at 2; reflexivity.
+Qed.
+Lemma pending_commands : forall (n:nat) (lc0 lc1 q:list cmd) (v0 v1:valuation),
+    In (SRunning v1 lc1) (do_steps n [SRunning v0 lc0])
+    -> In (SRunning v1 (lc1 ++ q)) (do_steps n [SRunning v0 (lc0 ++ q)]).
+Proof.
+  intro n; elim n; clear n.
+  (* Base case *)
+    intros lc0 lc1 q v0 v1 H; elim H; clear H.
+      intro eq; invert eq; exact (or_introl (eq_refl _)).
+      intro absurd; elim absurd.
+  (* Recursion *)
+    intros n rec lc0; elim lc0; clear lc0.
+    (* No command *)
+      intros lc1 q v0 v1 absurd.
+      replace (do_steps (S n) [SRunning v0 []]) with (do_steps n [SDone (Terminated v0)])
+          in absurd by reflexivity.
+      elim (small_terminated_only_terminated _ _
+          (terminated_future [SDone (Terminated v0)] (do_steps n [SDone (Terminated v0)])
+             (eq_refl _) (do_steps_ex _ _)) absurd).
+      discriminate.
+    intro a; elim a; clear a.
+    (* Assign *)
+      exact (fun _ _ _ _ _ _ _ _ => rec _ _ _ _ _).
+    (* Skip *)
+      exact (fun _ _ _ _ _ _ => rec _ _ _ _ _).
+    (* Seq *)
+      exact (fun _ _ _ _ _ _ _ _ _ _ => rec _ _ _ _ _).
+    (* Choose *)
+      intros c1 rec1 c2 rec2 l recl lc1 q v0 v1.
+      replace (((c1 <|> c2)%cmd :: l) ++ q)
+          with ((c1 <|> c2)%cmd :: (l ++ q)) by exact (eq_sym (app_comm_cons _ _ _)).
+      replace (do_steps (S n) [SRunning v0 ((c1 <|> c2)%cmd :: l)])
+          with (do_steps n ([SRunning v0 (c1::l)] ++ [SRunning v0 (c2::l)])) by reflexivity.
+      replace (do_steps (S n) [SRunning v0 ((c1 <|> c2)%cmd :: l ++ q)])
+          with (do_steps n ([SRunning v0 (c1::l++q)] ++ [SRunning v0 (c2::l++q)])) by reflexivity.
+      rewrite (step_split n _ _); rewrite (step_split n _ _).
+      intro H; elim (proj1 (in_app_iff _ _ _) H); clear H; intro H.
+        refine (proj2 (in_app_iff _ _ _) (or_introl (rec _ _ _ _ _ H))).
+        refine (proj2 (in_app_iff _ _ _) (or_intror (rec _ _ _ _ _ H))).
+    (* If *)
+      intros a c1 rec1 c2 rec2 l recl lc1 q v0 v1.
+      replace (((if_ a then c1 else c2)%cmd :: l) ++ q)
+          with ((if_ a then c1 else c2)%cmd :: (l ++ q)) by exact (eq_sym (app_comm_cons _ _ _)).
+      replace (do_steps (S n) [SRunning v0 ((if_ a then c1 else c2)%cmd :: l)])
+          with (do_steps n (
+            match interp a v0 with
+            | O => [SRunning v0 (c2::l)]
+            | _ => [SRunning v0 (c1::l)]
+            end ++ [])) by reflexivity; rewrite app_nil_r.
+      replace (do_steps (S n) [SRunning v0 ((if_ a then c1 else c2)%cmd :: l++q)])
+          with (do_steps n (
+            match interp a v0 with
+            | O => [SRunning v0 (c2::l++q)]
+            | _ => [SRunning v0 (c1::l++q)]
+            end ++ [])) by reflexivity; rewrite app_nil_r.
+      elim (eval_dec (interp a v0)); [| intro eqex; elim eqex; intro p];
+          intro eval; rewrite eval; exact (rec _ _ _ _ _).
+    (* While *)
+      intros a c recc l recl lc1 q v0 v1.
+      replace (((while a do c)%cmd :: l) ++ q)
+          with ((while a do c)%cmd :: (l ++ q)) by exact (eq_sym (app_comm_cons _ _ _)).
+      replace (do_steps (S n) [SRunning v0 ((while a do c)%cmd :: l)])
+          with (do_steps n (
+            match interp a v0 with
+            | O => [SRunning v0 l]
+            | _ => [SRunning v0 (c::(While a c)::l)]
+            end ++ [])) by reflexivity; rewrite app_nil_r.
+      replace (do_steps (S n) [SRunning v0 ((while a do c)%cmd :: l ++ q)])
+          with (do_steps n (
+            match interp a v0 with
+            | O => [SRunning v0 (l++q)]
+            | _ => [SRunning v0 (c::(While a c)::l++q)]
+            end ++ [])) by reflexivity; rewrite app_nil_r.
+      elim (eval_dec (interp a v0)); [| intro eqex; elim eqex; intro p];
+          intro eval; rewrite eval; exact (rec _ _ _ _ _).
+    (* Abort *)
+      intros l recl lc1 q v0 v1 absurd.
+      replace (do_steps (S n) [SRunning v0 (Abort :: l)])
+          with (do_steps n [SDone Aborted]) in absurd by reflexivity.
+      rewrite (abort_const n) in absurd.
+      elim absurd; clear absurd; [ discriminate | intro absurd; elim absurd ].
+Qed.
+
+Lemma split_computation0 : forall (lst1:state) (st1:singular_state),
+    In st1 lst1 -> forall (m:nat) (st2:singular_state), In st2 (do_steps m [st1]) -> In st2 (do_steps m lst1).
+Proof.
+  intro lst1; elim lst1; clear lst1.
+  (* [] *)
+    intros st1 absurd; elim absurd.
+  (* a::q *)
+    intros a q rec st1 H; replace (a::q) with ([a] ++ q) by reflexivity; elim H; clear H.
+    (* a = st1 *)
+      intros a_eq m st2 H; rewrite a_eq.
+      rewrite (step_split _ _ _).
+      exact (in_or_app _ _ _ (or_introl H)).
+    (* In st1 q *)
+      intros st1q m st2 H.
+      rewrite (step_split _ _ _).
+      refine (in_or_app _ _ _ (or_intror _)).
+      exact (rec st1 st1q m st2 H).
+Qed.
+
+Theorem split_computation1 (n m:nat) (lst0:list singular_state) (st1 st2:singular_state) :
+    In st1 (do_steps n lst0)
+    -> In st2 (do_steps m [st1])
+    -> In st2 (do_steps (m+n) lst0).
+Proof.
+  rewrite <- (do_steps_split _ _ _).
+  exact (fun H => split_computation0 _ _ H _ _).
+Qed.
+
+Theorem split_computation2 (n m:nat) (v0 v1:valuation) (lc q:list cmd) (st2:singular_state) :
+    In (SRunning v1 nil) (do_steps n [SRunning v0 lc])
+    -> In st2 (do_steps m [SRunning v1 q])
+    -> In st2 (do_steps (m+n) [SRunning v0 (lc ++ q)]).
+Proof (fun H => split_computation1 _ _ _ _ _ (pending_commands _ _ _ _ _ _ H)).
+
+Theorem big_to_small :
+    forall (v:valuation) (c:cmd) (r:result), eval v c r -> exists n:nat, In (SDone r) (do_steps n (init v c)).
+Proof.
+  assert (forall m:nat, m<>0 -> exists p:nat, m=S p) as intro_prec.
+    intro m; elim m; clear m.
+      intro absurd; elim (absurd (eq_refl O)).
+      exact (fun p _ _ => ex_intro _ p (eq_refl (S p))).
+  assert (forall (mv0 mv1:valuation) (mc:cmd), ~ In (SDone (Terminated mv1)) (init mv0 mc)) as cmd_takes_time.
+    intros mv0 mv1 mc absurd; elim absurd; clear absurd; intro absurd; [ discriminate absurd | elim absurd ].
+  intros v c r eval; elim eval.
+  (* EvalAssign *)
+    exact (fun _ _ _ => ex_intro _ 2 (in_eq _ nil)).
+  (* EvalSkip *)
+    exact (fun _ => ex_intro _ 2 (in_eq _ nil)).
+  (* EvalSeqAborted *)
+    intros v0 cmd0 cmd1 useless H; elim H; intro n; exists (S n).
+    replace (do_steps (S n) (init v0 (cmd0;; cmd1)%cmd))
+        with (do_steps n [SRunning v0 [cmd0; cmd1]]) by reflexivity.
+    exact (abort_interrupts _ _ _ _ H0).
+  (* EvalSeqSuccess *)
+    intros v0 cmd0 v1 cmd1 res cmd0eval rec0 cmd1eval rec1.
+    elim rec0; elim rec1; intros n0 rec0n n2 rec2n.
+    elim (before_termination _ _ _ (cmd_takes_time _ _ _) rec2n); intros n1 rec1n.
+    exists (S (n0 + n1)).
+    exact (split_computation2 _ _ _ _ _ _ _ rec1n rec0n).
+  (* EvalChoose0 *)
+    intros v0 cmd0 cmd1 res cmd0eval rec; elim rec; clear rec; intros n rec; exists (S n).
+    replace (do_steps (S n) (init v0 (cmd0 <|> cmd1)%cmd))
+        with (do_steps n ([SRunning v0 [cmd0]] ++ [SRunning v0 [cmd1]])) by reflexivity.
+    rewrite (step_split _ _ _).
+    exact (in_or_app _ _ _ (or_introl rec)).
+  (* EvalChoose1 *)
+    intros v0 cmd0 cmd1 res cmd0eval rec; elim rec; clear rec; intros n rec; exists (S n).
+    replace (do_steps (S n) (init v0 (cmd0 <|> cmd1)%cmd))
+        with (do_steps n ([SRunning v0 [cmd0]] ++ [SRunning v0 [cmd1]])) by reflexivity.
+    rewrite (step_split _ _ _).
+    exact (in_or_app _ _ _ (or_intror rec)).
+  (* EvalIfFalse *)
+    intros v0 a cmd1 cmd0 res interpeval cmd0eval rec; elim rec; clear rec; intros n rec; exists (S n).
+    replace (do_steps (S n) (init v0 (if_ a then cmd1 else cmd0)%cmd))
+        with (do_steps n (
+          match interp a v0 with
+          | O => [SRunning v0 [cmd0]]
+          | _ => [SRunning v0 [cmd1]]
+          end ++ [])) by reflexivity.
+    rewrite interpeval.
+    exact rec.
+  (* EvalIfTrue *)
+    intros v0 a cmd1 cmd0 res interpeval cmd1eval rec; elim rec; clear rec; intros n rec; exists (S n).
+    elim (intro_prec _ interpeval); clear interpeval; intros p interpeval.
+    replace (do_steps (S n) (init v0 (if_ a then cmd1 else cmd0)%cmd))
+        with (do_steps n (
+          match interp a v0 with
+          | O => [SRunning v0 [cmd0]]
+          | _ => [SRunning v0 [cmd1]]
+          end ++ [])) by reflexivity.
+    rewrite interpeval.
+    exact rec.
+  (* EvalWhileFalse *)
+    intros v0 a cmd0 interpeval; exists 2.
+    replace (do_steps 2 (init v0 (while a do cmd0)%cmd))
+        with (do_steps 1 (
+          match interp a v0 with
+          | O => [SRunning v0 nil]
+          | _ => [SRunning v0 [cmd0; While a cmd0]]
+          end ++ [])) by reflexivity.
+    rewrite interpeval.
+    exact (or_introl (eq_refl _)).
+  (* EvalWhileTrueAborted *)
+    intros v0 a cmd0 interpeval cmd0eval rec; elim rec; clear rec; intros n rec; exists (S n).
+    elim (intro_prec _ interpeval); clear interpeval; intros p interpeval.
+    replace (do_steps (S n) (init v0 (while a do cmd0)%cmd))
+        with (do_steps n (
+          match interp a v0 with
+          | O => [SRunning v0 nil]
+          | _ => [SRunning v0 [cmd0; While a cmd0]]
+          end ++ [])) by reflexivity.
+    rewrite interpeval.
+    exact (abort_interrupts _ _ _ _ rec).
+  (* EvalWhileTrueSuccess *)
+    intros v0 a cmd0 v1 res interpeval cmd0eval rec0 followeval followrec.
+    elim rec0; elim followrec; clear rec0 followrec; intros m followrec n rec0.
+    elim (intro_prec _ interpeval); clear interpeval; intros p interpeval.
+    elim (before_termination _ _ _ (cmd_takes_time _ _ _) rec0); intros n0 rec00.
+    exists (S (m+n0)).
+    replace (do_steps (S (m + n0)) (init v0 (while a do cmd0)%cmd))
+        with (do_steps (m + n0) (
+          match interp a v0 with
+          | O => [SRunning v0 nil]
+          | _ => [SRunning v0 [cmd0; While a cmd0]]
+          end ++ [])) by reflexivity.
+    rewrite interpeval.
+    exact (split_computation2 _ _ _ _ _ _ _ rec00 followrec).
+  (* EvalAbort *)
+    exact (fun _ => ex_intro _ 1 (or_introl (eq_refl _))).
+Qed.
+
+Lemma tail_cmd_unchanged : forall a v0 v1 q lc,
+    In (SRunning v1 lc) (full_step [SRunning v0 (a::q)])
+    -> exists lc1,
+      lc = lc1++q
+      /\
+      forall q', In (SRunning v1 (lc1++q')) (full_step [SRunning v0 (a::q')]).
+Proof.
+  intro a; elim a; clear a.
+  (* Assign *)
+    intros s a v0 v1 q lc H; invert H; invert H0.
+    exact (ex_intro _ nil (conj (eq_sym (app_nil_l lc)) (fun _ => or_introl (eq_refl _)))).
+  (* Skip *)
+    intros v0 v1 q lc H; invert H; invert H0.
+    exact (ex_intro _ nil (conj (eq_sym (app_nil_l lc)) (fun _ => or_introl (eq_refl _)))).
+  (* Seq *)
+    intros c1 rec1 c2 rec2 v0 v1 q lc H; invert H; invert H0.
+    exact (ex_intro _ [c1;c2] (conj (eq_refl _) (fun _ => or_introl (eq_refl _)))).
+  (* Choose *)
+    intros c1 rec1 c2 rec2 v0 v1 q lc H; invert H; invert H0; [| invert H | invert H ].
+    exact (ex_intro _ [c1] (conj (eq_refl _) (fun _ => or_introl (eq_refl _)))).
+    exact (ex_intro _ [c2] (conj (eq_refl _) (fun _ => or_intror (or_introl (eq_refl _))))).
+  (* If *)
+    intros a c1 rec1 c2 rec2 v0 v1 q lc.
+    replace (full_step [SRunning v0 ((if_ a then c1 else c2)%cmd :: q)]) with (
+        match interp a v0 with
+        | O => [SRunning v0 (c2::q)]
+        | _ => [SRunning v0 (c1::q)]
+        end ++ []) by reflexivity.
+    elim (eval_dec (interp a v0)); intro interpeval.
+    (* False *)
+      rewrite interpeval; intro H; invert H; invert H0.
+      refine (ex_intro _ [c2] (conj (eq_refl _) _)); intro q'.
+      replace (full_step [SRunning v1 ((if_ a then c1 else c2)%cmd :: q')]) with (
+          match interp a v1 with
+          | O => [SRunning v1 (c2::q')]
+          | _ => [SRunning v1 (c1::q')]
+          end ++ []) by reflexivity.
+      rewrite interpeval; exact (or_introl (eq_refl _)).
+    (* True *)
+      elim interpeval; clear interpeval; intros p interpeval.
+      rewrite interpeval; intro H; invert H; invert H0.
+      refine (ex_intro _ [c1] (conj (eq_refl _) _)); intro q'.
+      replace (full_step [SRunning v1 ((if_ a then c1 else c2)%cmd :: q')]) with (
+          match interp a v1 with
+          | O => [SRunning v1 (c2::q')]
+          | _ => [SRunning v1 (c1::q')]
+          end ++ []) by reflexivity.
+      rewrite interpeval; exact (or_introl (eq_refl _)).
+  (* While *)
+    intros a c rec v0 v1 q lc.
+    replace (full_step [SRunning v0 ((while a do c)%cmd :: q)]) with (
+        match interp a v0 with
+        | O => [SRunning v0 q]
+        | _ => [SRunning v0 (c::While a c::q)]
+        end ++ []) by reflexivity.
+    elim (eval_dec (interp a v0)); intro interpeval.
+    (* False *)
+      rewrite interpeval; intro H; invert H; invert H0.
+      refine (ex_intro _ nil (conj (eq_refl _) _)); intro q'.
+      replace (full_step [SRunning v1 ((while a do c)%cmd :: q')]) with (
+          match interp a v1 with
+          | O => [SRunning v1 q']
+          | _ => [SRunning v1 (c::While a c::q')]
+          end ++ []) by reflexivity.
+      rewrite interpeval; exact (or_introl (eq_refl _)).
+    (* True *)
+      elim interpeval; clear interpeval; intros p interpeval.
+      rewrite interpeval; intro H; invert H; invert H0.
+      refine (ex_intro _ [c; (While a c)] (conj (eq_refl _) _)); intro q'.
+      replace (full_step [SRunning v1 ((while a do c)%cmd :: q')]) with (
+          match interp a v1 with
+          | O => [SRunning v1 q']
+          | _ => [SRunning v1 (c::(While a c)::q')]
+          end ++ []) by reflexivity.
+      rewrite interpeval; exact (or_introl (eq_refl _)).
+  (* Abort *)
+    intros v0 v1 q lc absurd; elim absurd; clear absurd; [ discriminate | intro absurd; elim absurd ].
+Qed.
+
+Theorem code_split : forall (n:nat) (st:singular_state) (lc1 lc2:list cmd) (v:valuation),
+    In st (do_steps n [SRunning v (lc1 ++ lc2)]) -> 
+      (
+        (* c1 terminates in n steps *)
+        exists (v2:valuation) (m:nat),
+        m<=n
+        /\ In (SDone (Terminated v2)) (do_steps n [SRunning v lc1])
+        /\ In st (do_steps m [SRunning v2 lc2])
+      ) \/ (
+        (* c1 does not terminate in n steps *)
+        exists st0:singular_state,
+        (
+          (st = SDone Aborted /\ st0 = st)
+          \/
+          (exists v0 l0, st = SRunning v0 (l0 ++ lc2) /\ st0 = SRunning v0 l0)
+        )
+        /\ In st0 (do_steps n [SRunning v lc1])
+      ).
+Proof.
+  assert (forall s v, In (SDone (Terminated v)) s -> In (SDone (Terminated v)) (full_step s))
+      as terminated_const.
+    intro s; elim s; clear s; [ intros v H; elim H |].
+    intros a q rec v H; elim H; clear H.
+    (* Head *)
+      intro a_eq; rewrite a_eq.
+      replace (full_step (SDone (Terminated v) :: q))
+          with (flat_map singular_step ([SDone (Terminated v)] ++ q)) by reflexivity.
+      rewrite (flat_map_app _ _ singular_step _ _).
+      exact (or_introl (eq_refl _)).
+    (* Tail *)
+      replace (full_step (a :: q))
+          with (flat_map singular_step ([a] ++ q)) by reflexivity.
+      rewrite (flat_map_app _ _ singular_step _ _).
+      exact (fun P => in_or_app _ _ _ (or_intror (rec _ P))).
+  intro n; elim n; clear n.
+  (* Base case *)
+    intros st lc1 lc2 v H; elim H; [| intro absurd; elim absurd ]; clear H.
+    intro st_val; rewrite <- st_val; clear st_val; right.
+    exists (SRunning v lc1); refine (conj _ (or_introl (eq_refl _))).
+    right; exists v, lc1; exact (conj (eq_refl _) (eq_refl _)).
+  (* Recursion *)
+    intros n rec st lc1 lc2 v H.
+    replace (do_steps (S n) [SRunning v (lc1 ++ lc2)])
+        with (do_steps n (full_step [SRunning v (lc1 ++ lc2)])) in H by reflexivity.
+    rewrite <- (do_steps_split0 n _) in H.
+    destruct st.
+    (* st = SRunning v0 l *)
+      elim (before_running _ _ _ H); clear H; intros v4 H; elim H; clear H; intros lc4 [H1 H2].
+      elim (rec _ _ _ _ H1); clear rec; intro H; elim H; clear H.
+      (* Left branch *)
+        intros v2 H; elim H; clear H; intros m [mcmp [nstep mstep]].
+        left; exists v2, (S m); refine (conj (le_n_S _ _ mcmp) _).
+        exact (conj
+            (split_computation1 n 1 _ _ _ nstep (or_introl (eq_refl _)))
+            (split_computation1 m 1 _ _ _ mstep H2)).
+      (* Right branch *)
+        intros st0 [H H3]; elim H; clear H; intro H; elim H; clear H; [ discriminate |].
+        intros vf H; elim H; clear H; intros l0 [H4 H5].
+        destruct l0.
+        (* Finishes in c1 after n+1 steps *)
+          destruct lc2; [ invert H4; elim H2; [ discriminate | intro absurd; elim absurd ] |].
+          rewrite (app_nil_l _) in H4; invert H4.
+          left; exists vf, 1; refine (conj (Nat.lt_0_succ n) (conj _ H2)).
+          exact (split_computation1 n 1 _ _ _ H3 (or_introl (eq_refl _))).
+        (* Does not finish in c1 *)
+          invert H4; right.
+          elim (tail_cmd_unchanged _ _ _ _ _ H2); intros hlc [l_eq H].
+          exists (SRunning v0 (hlc ++ l0)).
+          refine (conj (or_intror _) (split_computation1 n 1 _ _ _ H3 (H l0))).
+          exists v0, (hlc ++ l0); refine (conj _ (eq_refl _)).
+          rewrite l_eq, (app_assoc _ _ _); reflexivity.
+    destruct r.
+    (* st = SDone (Terminvated v0) *)
+      elim (before_termination_or _ _ H); clear H; intro H.
+      (* c1;;c2 finish after n *)
+        elim (rec _ _ _ _ H); clear rec; intro Hrec; elim Hrec; clear Hrec;
+            [| intros st0 [absurd H2]; invert absurd; [| invert H0; invert H1 ]; discriminate (proj1 H0) ].
+        intros v2 Hrec; elim Hrec; clear Hrec; intros m [m_le_n [nstep mstep]]; left.
+        exists v2, m; refine (conj (le_S m n m_le_n) (conj _ mstep)).
+        exact (split_computation1 n 1 _ _ _ nstep (or_introl (eq_refl))).
+      (* c1;;c2 finish at n+1 *)
+        elim (rec _ _ _ _ H); clear rec; intro Hrec; elim Hrec; clear Hrec.
+        (* Left branch *)
+          intros v2 Hrec; elim Hrec; clear Hrec; intros m [m_le_n [nstep mstep]].
+          left; exists v2, (S m); refine (conj (le_n_S _ _ m_le_n) _).
+          exact (conj
+              (split_computation1 n 1 _ _ _ nstep (or_introl (eq_refl)))
+              (split_computation1 m 1 _ _ _ mstep (or_introl (eq_refl)))).
+        (* Right branch *)
+          intros st0 [H1 H2]; invert H1; [ discriminate (proj1 H0) |].
+          elim H0; clear H0; intros v2 H0; elim H0; clear H0; intros m [sreq st0_eq].
+          invert st0_eq. invert sreq. pose (test := app_eq_nil _ _ (eq_sym H3)). invert test.
+          left; exists v2, 1; refine (conj (Nat.lt_0_succ n) (conj _ (or_introl (eq_refl _)))).
+          exact (split_computation1 n 1 _ _ _ H2 (or_introl (eq_refl _))).
+    (* st = SDone Aborted *)
+      elim (before_aborted _ H); clear H; intro H.
+      (* Aborted after n steps *)
+        elim (rec _ _ _ _ H); clear rec; intro Hrec; elim Hrec; clear Hrec.
+        (* Aborted in c2 after n steps *)
+          intros v2 Hrec; elim Hrec; clear Hrec; intros m [m_le_n [nstep mstep]]; left.
+          exists v2, m; refine (conj (le_S _ _ m_le_n) (conj _ mstep)).
+          exact (split_computation1 n 1 _ _ _ nstep (or_introl (eq_refl _))).
+        (* Aborted in c1 after n steps *)
+          intros st0 [H1 H2]; elim H1; clear H1; [| intro H1; invert H1; invert H0; discriminate (proj1 H1) ].
+          intros [useless st0_eq]; invert st0_eq; right; exists (SDone Aborted).
+          refine (conj (or_introl (conj (eq_refl _) (eq_refl _))) _).
+          exact (split_computation1 n 1 _ _ _ H2 (or_introl (eq_refl _))).
+      (* Aborted at n+1 steps *)
+        elim H; clear H; intros v0 H; elim H; clear H; intros q H.
+        elim (rec _ _ _ _ H); clear rec; intro Hrec; elim Hrec; clear Hrec.
+        (* c1 terminates after n steps *)
+          intros v2 Hrec; elim Hrec; clear Hrec; intros m [m_le_n [nstep mstep]].
+          left; exists v2, (S m); refine (conj (le_n_S _ _ m_le_n) _).
+          exact (conj
+              (split_computation1 n 1 _ _ _ nstep (or_introl (eq_refl)))
+              (split_computation1 m 1 _ _ _ mstep (or_introl (eq_refl)))).
+        (* c1 does not terminate after n steps *)
+          intros st0 [H1 H2]; elim H1; clear H1; [ intro absurd; discriminate (proj1 absurd) |].
+          intro H1; elim H1; clear H1; intros v1 H1; elim H1; clear H1; intros l0 [H1 st0_eq].
+          invert st0_eq; induct l0.
+          (* c1 terminates at n+1 steps *)
+            left; exists v1, 1; refine (conj (Nat.lt_0_succ n) _).
+            rewrite (app_nil_l _) in H1; rewrite <- H1.
+            exact (conj
+                (split_computation1 n 1 _ _ _ H2 (or_introl (eq_refl)))
+                (or_introl (eq_refl _))).
+          (* c1 aborts at n+1 steps *)
+            right; exists (SDone Aborted); refine (conj (or_introl (conj (eq_refl _) (eq_refl _))) _).
+            invert H1.
+            exact (split_computation1 n 1 _ _ _ H2 (or_introl (eq_refl _))).
+Qed.
+
+Lemma small_abort_big_may_abort_n : forall n:nat, forall v c r,
+    In (SDone r) (do_steps n (init v c)) -> eval v c r.
+Proof.
+  assert (forall (m:nat) (v:valuation),
+      do_steps m [SDone (Terminated v)] = [SDone (Terminated v)]) as termination_const.
+    intro m; elim m; clear m; [ reflexivity | exact (fun _ H => H) ].
+  assert (forall (n:nat) (v:valuation), In (SDone (Terminated v)) (do_steps n [SDone (Terminated v)])) as term_f.
+    intro n; elim n.
+      exact (fun v => or_introl (eq_refl _)).
+      exact (fun p rec v => split_computation1 p 1 _ _ _ (rec v) (or_introl (eq_refl))).
+  intro n; elim n; clear n.
+  (* Base case *)
+    intros v c r absurd; elim absurd; clear absurd; [ discriminate | intro absurd; elim absurd ].
+  (* Recursion *)
+    intros n rec v c; elim c; clear c.
+    (* Assign *)
+      intros s a r.
+      destruct n; [ intro absurd; elim absurd; clear absurd; intro absurd; [ discriminate | elim absurd ] |].
+      replace (do_steps (S (S n)) (init v (s <- a)%cmd))
+          with (do_steps n [SDone (Terminated (v $+ (s, interp a v)))]) by reflexivity.
+      rewrite (termination_const n _).
+      intro H; elim H; clear H; intro H; invert H.
+      exact (EvalAssign _ _ _).
+    (* Skip *)
+      destruct n; [ intros r absurd; elim absurd; clear absurd; [ discriminate | intro absurd; elim absurd ] |].
+      replace (do_steps (S (S n)) (init v Skip))
+          with (do_steps n [SDone (Terminated v)]) by reflexivity.
+      rewrite (termination_const n v).
+      intro H; elim H; clear H.
+        intros v0 H; elim H; clear H.
+          intro H; invert H; exact (EvalSkip _).
+          intro H; elim H.
+        intro absurd; elim absurd; clear absurd; [ discriminate | intro absurd; elim absurd ].
+    (* Seq *)
+      intros c1 rec1 c2 rec2 r.
+      replace (do_steps (S n) (init v (c1;; c2)%cmd))
+          with (do_steps n [SRunning v [c1; c2]]) by reflexivity.
+      elim r; clear r.
+      (* Terminated v0 *)
+        intros v0 H; elim (code_split n _ [c1] [c2] v H); clear H.
+        (* Left branch *)
+          intro H2; elim H2; clear H2; intros v2 H2; elim H2; clear H2; intros m [m_le_n [nstep mstep]].
+          refine (EvalSeqSuccess v c1 v2 c2 (Terminated v0) (rec _ _ _ nstep) (rec _ _ _ _)).
+          rewrite (le_plus_minus _ _ m_le_n), (plus_comm _ _).
+          exact (split_computation1 m (n - m) _ _ _ mstep (term_f _ v0)).
+        (* Right branch - absurd *)
+          intro H2; elim H2; clear H2; intros st0 [H2 nstep]; elim H2; clear H2; intro H2;
+            [ discriminate (proj1 H2) | invert H2; invert H; discriminate (proj1 H0) ].
+      (* Aborted *)
+        intro H; elim (code_split n _ [c1] [c2] v H); clear H.
+        (* Left branch *)
+          intro H2; elim H2; clear H2; intros v2 H2; elim H2; clear H2; intros m [m_le_n [nstep mstep]].
+          refine (EvalSeqSuccess v c1 v2 c2 Aborted (rec _ _ _ nstep) (rec _ _ _ _)).
+          rewrite (le_plus_minus _ _ m_le_n), (plus_comm _ _).
+          refine (split_computation1 m (n - m) _ _ _ mstep _).
+          rewrite (abort_const (n - m)); exact (or_introl (eq_refl _)).
+        (* Right branch *)
+          intro H2; elim H2; clear H2; intros st0 [H2 nstep]; elim H2; clear H2; intro H2;
+            [| invert H2; invert H; discriminate (proj1 H0) ].
+          invert H2; destruct H.
+          exact (EvalSeqAborted _ _ _ (rec _ _ _ nstep)).
+    (* Choose *)
+      intros c1 rec1 c2 rec2 r.
+      replace (do_steps (S n) (init v (c1 <|> c2)%cmd))
+          with (do_steps n ([SRunning v [c1]] ++ [SRunning v [c2]])) by reflexivity.
+      rewrite (step_split n _ _).
+      intro H; elim (in_app_or _ _ _ H); clear H; intro H.
+      (* Result from c1 *)
+        exact (EvalChoose0 v c1 c2 r (rec _ _ _ H)).
+      (* Result from c2 *)
+        exact (EvalChoose1 v c1 c2 r (rec _ _ _ H)).
+    (* If *)
+      intros a c1 rec1 c2 rec2 r.
+      replace (do_steps (S n) (init v (if_ a then c1 else c2)%cmd))
+          with (do_steps n (
+            match interp a v with
+            | O => [SRunning v [c2]]
+            | _ => [SRunning v [c1]]
+            end ++ [])) by reflexivity.
+      elim (eval_dec (interp a v)); intros interpeval H.
+      (* False branch *)
+        rewrite interpeval in H.
+        exact (EvalIfFalse v a c1 c2 r interpeval (rec _ _ _ H)).
+      (* True branch *)
+        elim interpeval; clear interpeval; intros p interpeval.
+        assert (interp a v <> O) as condition_true; [ rewrite interpeval; discriminate |].
+        rewrite interpeval in H.
+        exact (EvalIfTrue v a c1 c2 r condition_true (rec _ _ _ H)).
+    (* While *)
+      intros a c recc r.
+      replace (do_steps (S n) (init v (while a do c)%cmd))
+          with (do_steps n (
+            match interp a v with
+            | O => [SRunning v []]
+            | _ => [SRunning v [c; While a c]]
+            end ++ [])) by reflexivity.
+      elim (eval_dec (interp a v)); intros interpeval H.
+      (* False branch *)
+        rewrite interpeval in H.
+        destruct n; [ invert H; [ discriminate H0 | invert H0 ] |].
+        replace (do_steps (S n) ([SRunning v []] ++ []))
+            with (do_steps n [SDone (Terminated v)]) in H by reflexivity.
+        rewrite (termination_const n v) in H; invert H; invert H0.
+        exact (EvalWhileFalse v a c interpeval).
+      (* True branch *)
+        elim interpeval; clear interpeval; intros p interpeval.
+        assert (interp a v <> O) as condition_true; [ rewrite interpeval; discriminate |].
+        rewrite interpeval in H.
+        replace ([SRunning v [c; (while a do c)%cmd]] ++ [])
+            with ([SRunning v ([c] ++ [(while a do c)%cmd])]) in H by reflexivity.
+        elim (code_split _ _ _ _ _ H); clear H; intro H; elim H; clear H.
+        (* c terminates *)
+          intros v2 H; elim H; clear H; intros m [m_le_n [nstep mstep]].
+          refine (EvalWhileTrueSuccess v a c v2 r condition_true (rec _ _ _ nstep) (rec _ _ _ _)).
+          rewrite (le_plus_minus _ _ m_le_n), (plus_comm _ _).
+          refine (split_computation1 m (n - m) _ _ _ mstep _).
+          destruct r; [ rewrite (termination_const _ _) | rewrite (abort_const _) ];
+              exact (or_introl (eq_refl _)).
+        (* c aborts *)
+          intros st0 [H nstep]; elim H; clear H; intro H;
+              [| invert H; invert H0; discriminate (proj1 H) ].
+          invert H; invert H0.
+          exact (EvalWhileTrueAborted v a c condition_true (rec _ _ _ nstep)).
+    (* Abort *)
+      replace (do_steps (S n) (init v Abort)) with (do_steps n [SDone Aborted]) by reflexivity.
+      rewrite (abort_const _); intros r H; invert H; invert H0.
+      exact (EvalAbort v).
+Qed.
+
 Theorem small_abort_big_may_abort : forall v c s,
          step^* (init v c) s
       -> small_aborted s
       -> exists res, eval v c res /\ big_aborted res.
 Proof.
-Admitted.
-
-
+  intros v c s evol; elim (do_steps_find _ _ evol); clear evol; intros n s_eq; invert s_eq.
+  Check small_abort_big_may_abort_n.
+  exact (fun H => ex_intro _ Aborted (conj (small_abort_big_may_abort_n n v c Aborted H) (eq_refl _))).
+Qed.
 
 (* As an additional challenge, you  you may want to prove the following
  * theorem. Note that this is *NOT* required for this assignment and
@@ -269,7 +1672,15 @@ Admitted.
  *
  * If the small-step semantics terminates without aborting, then the
  * big-step semantics may *not* abort.
-
+ *)
+Lemma le_exists (n m:nat) : n <= m \/ m <= n.
+Proof.
+  cases (n ?= m).
+    rewrite (proj1 (Nat.compare_eq_iff _ _) Heq); exact (or_introl (le_n _)).
+    exact (or_introl (le_S_n _ _ (le_S _ _ (proj1 (Nat.compare_lt_iff _ _) Heq)))).
+    refine (or_intror (le_S_n _ _ (le_S _ _ (proj1 (Nat.compare_lt_iff _ _) _))));
+        rewrite (Nat.compare_antisym _ _), Heq; reflexivity.
+Qed.
 Theorem small_terminates_big_may_not_abort :
        forall v c s,
          step^* (init v c) s
@@ -279,5 +1690,22 @@ Theorem small_terminates_big_may_not_abort :
           -> big_aborted res
           -> False.
 Proof.
-Admitted.
-*)
+  intros v c s small_evol term_s r big_evol r_abort; invert r_abort.
+  elim (big_to_small v c _ big_evol); intros n small_abort.
+  elim (do_steps_find _ _ small_evol); clear small_evol; intros m small_term; invert small_term.
+  elim (le_exists n m).
+  (* n <= m *)
+    intro n_le_m.
+    assert (In (SDone Aborted) (do_steps m (init v c))) as combined_aborted.
+      rewrite (le_plus_minus _ _ n_le_m), (plus_comm _ _).
+      refine (split_computation1 _ (m - n) _ _ (SDone Aborted) small_abort _).
+      rewrite (abort_const _); exact (or_introl (eq_refl _)).
+    exact (terminated_not_aborted _ term_s combined_aborted).
+  (* m <= n *)
+    intro m_le_n.
+    assert (small_terminated (do_steps n (init v c))) as combined_term.
+      rewrite (le_plus_minus _ _ m_le_n), (plus_comm _ _).
+      rewrite <- (do_steps_split _ _ _).
+      exact (terminated_future _ _ term_s (do_steps_ex (n - m) _)).
+    exact (terminated_not_aborted _ combined_term small_abort).
+Qed.
